WIP trace proofs

aneris/examples/transactional_consistency/read_committed/trace/trace_proof.v
@@ -2,7 +2,7 @@ From iris.algebra Require Import gset auth gmap excl excl_auth csum.
 From iris.base_logic.lib Require Import mono_nat ghost_map.
 From iris.algebra.lib Require Import mono_list.
 From aneris.algebra Require Import monotone.
-From aneris.aneris_lang Require Import network resources proofmode.
+From aneris.aneris_lang Require Import network resources proofmode adequacy_no_model.
 From aneris.lib Require Import gen_heap_light.
 From aneris.aneris_lang.lib Require Import list_proof inject lock_proof.
 From aneris.aneris_lang.lib.serialization Require Import serialization_proof.
@@ -12,10 +12,10 @@ From aneris.examples.transactional_consistency.read_committed.specs Require Impo
 From aneris.examples.transactional_consistency Require Import user_params aux_defs state_based_model.
 
 Section trace_proof.
-  Context `{!anerisG Mdl Σ, !User_params}.
+  Context `{!User_params}.
 
   (** Wrapped resources  *)
-  Global Program Instance wrapped_resources `(res : !RC_resources Mdl Σ) : RC_resources Mdl Σ :=
+  Global Program Instance wrapped_resources `{!anerisG Mdl Σ} `(res : !RC_resources Mdl Σ) : RC_resources Mdl Σ :=
     {|
       GlobalInv := True%I;
       OwnMemKey k V := True%I;
@@ -36,27 +36,14 @@ Section trace_proof.
   Next Obligation.
   Admitted.
 
-  (* Library specification on the form required by the trace infrastructure *)
-  Definition rc_library_spec (clients : gset socket_address) (P0 : iProp Σ) 
-  (lib : KVS_transaction_api) : iProp Σ := 
-      (P0 -∗ ∃ (res : RC_resources Mdl Σ),
-               ([∗ set] k ∈ KVS_keys, k ↦ₖ ∅) ∗ 
-               KVS_Init ∗ 
-               GlobalInv ∗
-               ([∗ set] sa ∈ clients, KVS_ClientCanConnect sa) ∗
-               init_kvs_spec ∗
-               init_client_proxy_spec ∗
-               read_spec ∗
-               write_spec ∗
-               start_spec ∗
-               commit_spec).
+  Definition trace_inv_name := nroot.@"trinv".
 
   (* Primary lemma to be used with adequacy *)
-  Lemma library_implication (clients : gset socket_address) 
-  (N : namespace) (P0 : iProp Σ) (lib : KVS_transaction_api) :
-    rc_library_spec clients P0 lib -∗
-    rc_library_spec clients (P0 ∗ trace_is [] ∗ trace_inv N valid_trace_rc) 
-                            (KVS_wrapped_api lib).
+  Lemma library_implication `{!anerisG Mdl Σ} (clients : gset socket_address) 
+  (lib : KVS_transaction_api) :
+    ((RC_spec clients lib) ∗
+    trace_is [] ∗ trace_inv trace_inv_name valid_trace_rc) ={⊤}=∗ 
+    RC_spec clients (KVS_wrapped_api lib).
   Proof.
   Admitted.
 
