aneris/examples/transactional_consistency/read_committed/examples/trace_proof_of_concept/trace_proof_of_concept_code.v
@@ -1,0 +1,30 @@
+From aneris.aneris_lang Require Import ast.
+From aneris.aneris_lang.lib.serialization Require Import serialization_code.
+From aneris.examples.transactional_consistency.snapshot_isolation Require Import snapshot_isolation_code.
+From aneris.examples.transactional_consistency Require Import wrapped_library.
+From aneris.examples.transactional_consistency.snapshot_isolation.util Require Import util_code.
+
+Definition transaction1 : val :=
+  λ: "cst", (wrap_start start) "cst";;
+             (wrap_write write) "cst" #"x" #1;;
+             loop #().
+
+Definition transaction2 : val :=
+  λ: "cst",
+  (wrap_start start) "cst";;
+  let: "vx" := (wrap_read read) "cst" #"x" in
+  assert: ("vx" = NONE);;
+  (wrap_commit commit) "cst" ;;
+  #().
+
+Definition transaction1_client : val :=
+  λ: "caddr" "kvs_addr",
+  let: "cst" := init_client_proxy int_serializer "caddr" "kvs_addr" in
+  transaction1 "cst".
+
+Definition transaction2_client : val :=
+  λ: "caddr" "kvs_addr",
+  let: "cst" := init_client_proxy int_serializer "caddr" "kvs_addr" in
+  transaction2 "cst".
+
+Definition server : val := λ: "srv", init_server int_serializer "srv".
